examples/Imp2Vir/Semantics.v
@@ -1,5 +1,6 @@
 From Coq Require Import
      Lia
+     List
      String
      ZArith.
 
@@ -14,25 +15,11 @@ From Vellvm Require Import
      Semantics
      Syntax
      Syntax.ScopeTheory
+     Utils.AListFacts
      Utils.Tactics.
 From Imp2Vir Require Import Fin Imp.
 
-Require Import Vec Unique CvirCombinators CvirCombinatorsWF CompileExpr Imp2Cvir.
-
-Definition Rmem (env : Imp.env) (vmap : StringMap.t int) (venv : local_env) (vmem : memory_stack) : Prop :=
-  forall k v, alist_find k env = Some v <-> (
-    exists reg, StringMap.find k vmap = Some reg /\
-      exists addr, alist_find (Anon reg) venv = Some (UVALUE_Addr addr) /\
-        exists v32, read vmem addr (DTYPE_I (Npos 32%positive)) = inr (UVALUE_I32 v32) /\
-          Int32.intval v32 = Z.of_nat v
-  ).
-
-Definition Rimpvir
-  (vmap : StringMap.t int)
-  (env1 : Imp.env * unit)
-  (env2 : memory_stack * (local_env * (global_env * (block_id * block_id + uvalue)))) :
-  Prop :=
-  Rmem (fst env1) vmap (fst (snd env2)) (fst env2).
+From Imp2Vir Require Import Utils Relabel Vec Unique CvirCombinators CvirCombinatorsWF CompileExpr Imp2Cvir.
 
 (* Denotation of a [cvir] construct.
   Note: we should be able to take any three disjoint sets 
@@ -45,13 +32,20 @@ Definition Rimpvir
   necessary to express generic lemmas, even if "at the top level"
   we will always use the canonical naming. It is not yet clear though. 
 *)
+
+Definition denote_cvir_gen {ni no} (ir : cvir ni no) vi vo vt (bid bid' : fin ni) :=
+  denote_ocfg (convert_typ nil (blocks ir vi vo vt)) (nth vi bid', nth vi bid).
+
 Definition build_map a b :=
   map Anon (map Z.of_nat (seq a b)).
 
-Definition denote_cvir_gen {ni no} (ir : cvir ni no) vi vo vt (bid : fin ni) bid' :=
-  denote_ocfg (convert_typ nil (blocks ir vi vo vt)) (bid', nth vi bid).
+Definition blocks_default {ni no} (ir : cvir ni no) :=
+  let vi := build_map 0 ni in
+  let vo := build_map ni no in
+  let vt := build_map (ni + no) (n_int ir) in
+  blocks ir vi vo vt.
 
-Definition denote_cvir {ni no} (ir : cvir ni no) (bid : fin ni) bid' :=
+Definition denote_cvir {ni no} (ir : cvir ni no) bid bid' :=
   let vi := build_map 0 ni in
   let vo := build_map ni no in
   let vt := build_map (ni + no) (n_int ir) in
@@ -80,14 +74,28 @@ leads to some non-trivial arithmetic and reasoning on renaming.
 Maybe using this hypothetical higher level lemma could sooth the pain.
  *)
 
-(* The following lemmas should be true *)
 Lemma firstn_build_map : forall i n m,
 firstn n (build_map i (n + m)) = build_map i n.
-Admitted.
+Proof.
+  intros.
+  unfold firstn, build_map, seq, map.
+  apply vector_proj1_unique.
+  simpl.
+  rewrite !firstn_map.
+  f_equal. f_equal.
+  apply firstn_seq.
+Qed.
 
 Lemma skipn_build_map : forall i n m,
 skipn n (build_map i (n + m)) = build_map (i + n) m.
-Admitted.
+Proof.
+  intros.
+  apply vector_proj1_unique.
+  simpl.
+  rewrite !skipn_map.
+  do 2 f_equal.
+  apply skipn_seq.
+Qed.
 
 Lemma nth_build_map : forall i n k,
   nth (build_map i n) k = Anon (Z.of_nat(i + proj1_sig k)).
@@ -102,86 +110,200 @@ Proof.
   Unshelve. exact O.
 Qed.
 
+Lemma cvir_inputs_build_map : forall {ni no} ir fi fo ft n,
+  cvir_ids_WF ir ->
+  cvir_inputs_used ir ->
+  List.In (Anon (Z.of_nat n)) (inputs (blocks ir (build_map fi ni) (build_map fo no) (build_map ft (n_int ir)))) <->
+  (n >= fi /\ n < fi + ni)%nat \/ (n >= ft /\ n < ft + n_int ir)%nat.
+Proof.
+  split; intros.
+  - apply cvir_inputs in H1; try assumption.
+    apply List.in_app_iff in H1.
+    simpl in H1.
+    rewrite 2 List.map_map in H1.
+    setoid_rewrite List.in_map_iff in H1.
+    destruct H1 as [(? & ? & ?) | (? & ? & ?)];
+    inv H1;
+    apply Nat2Z.inj in H4; subst x;
+    apply List.in_seq in H2;
+    tauto.
+  - apply cvir_inputs; try assumption.
+    apply vector_in_app_iff.
+    cbn.
+    rewrite !List.map_map.
+    setoid_rewrite List.in_map_iff.
+    setoid_rewrite List.in_seq.
+    destruct H1; [ left | right ];
+    exists n;
+    tauto.
+Qed.
+
+Lemma cvir_outputs_build_map' : forall {ni no} ir fi fo ft o,
+  cvir_ids_WF ir ->
+  List.In o (outputs (blocks ir (build_map fi ni) (build_map fo no) (build_map ft (n_int ir)))) ->
+  exists n,
+    o = Anon (Z.of_nat n) /\
+    ((n >= fi /\ n < fi + ni)%nat \/ (n >= fo /\ n < fo + no)%nat \/ (n >= ft /\ n < ft + n_int ir)%nat).
+Proof.
+  intros.
+  unfold build_map in H0.
+  apply cvir_outputs in H0; try assumption.
+  cbn in H0.
+  rewrite !List.in_app_iff in H0.
+  rewrite !List.map_map in H0.
+  rewrite !List.in_map_iff in H0.
+  setoid_rewrite List.in_seq in H0.
+  destruct H0 as [(? & ? & ?) | [(? & ? & ?) | (? & ? & ?)]];
+  exists x; subst o;
+  tauto.
+Qed.
+
+Lemma cvir_outputs_build_map : forall {ni no} ir fi fo ft n,
+  cvir_ids_WF ir ->
+  List.In (Anon (Z.of_nat n)) (outputs (blocks ir (build_map fi ni) (build_map fo no) (build_map ft (n_int ir)))) ->
+  (n >= fi /\ n < fi + ni)%nat \/ (n >= fo /\ n < fo + no)%nat \/ (n >= ft /\ n < ft + n_int ir)%nat.
+Proof.
+  intros.
+  apply cvir_outputs_build_map' in H0; try assumption.
+  destruct H0 as (? & ? & ?). inv H0.
+  apply Nat2Z.inj in H3. subst x.
+  tauto.
+Qed.
+
 From Coq Require Import Morphisms.
 Require Import ITree.Basics.HeterogeneousRelations.
 Import ITreeNotations.
-Import SemNotations.
+(*Import SemNotations.*)
 
-Lemma find_block_map_some' :
-  forall {T T'} (f : block T -> block T') G b bk,
-    (forall bk, blk_id (f bk) = blk_id bk) ->
-    find_block G b = Some bk ->
-    find_block (List.map f G) b = Some (f bk).
-Proof.
-  intros * ID; induction G as [| hd G IH]; intros FIND ; [inv FIND |].
-  cbn in *.
-  rewrite ID. 
-  break_match_goal; break_match_hyp; intuition.
-  inv FIND; auto.
-Qed.
+Definition vec_build_map {A n} (v v' : Vec.t A n) : alist A A :=
+  List.combine (proj1_sig v) (proj1_sig v').
 
-Lemma find_block_map_none' :
-  forall {T T'} (f : block T -> block T') G b,
-    (forall bk, blk_id (f bk) = blk_id bk) ->
-    find_block G b = None ->
-    find_block (List.map f G) b = None.
-Proof.
-  intros * ID; induction G as [| hd G IH]; intros FIND; [reflexivity |].
-  cbn in *.
-  rewrite ID. 
-  break_match_goal; break_match_hyp; intuition.
-  inv FIND; auto.
-Qed.
+(* TODO move to CvirCombinatorsWF.v *)
+Definition cvir_relabel_WF {ni no} (ir : cvir ni no) :=
+  forall vi vi' vo vo' vt vt',
+  unique_vector (vi ++ vo ++ vt) ->
+  unique_vector (vi' ++ vo' ++ vt') ->
+  blocks ir vi' vo' vt' =
+  ocfg_relabel (vec_build_map (vi++vo++vt) (vi'++vo'++vt')) (blocks ir vi vo vt).
 
-Lemma find_block_map' :
-  forall {T T'} (f : block T -> block T') G b,
-    (forall bk, blk_id (f bk) = blk_id bk) ->
-    find_block (List.map f G) b = option_map f (find_block G b).
-Proof.
-  intros.
-  destruct (find_block G b) eqn:EQ.
-  eapply find_block_map_some' in EQ; eauto.
-  eapply find_block_map_none' in EQ; eauto.
-Qed.
-
-(* This convenient lemma is not true. *)
-Lemma cvir_inputs_used :
-  forall {ni no} (ir : cvir ni no) vi vo vt bid,
-  cvir_ids_WF ir ->
-  In bid (vi ++ vt) -> List.In bid (inputs (blocks ir vi vo vt)).
+Lemma unique_vector_split6 :
+  forall A n1 n2 n3 n4 n5 n6 v1 v2 v3 v4 v5 v6,
+  unique_vector ((v1 ++ v2) ++ (v3 ++ v4) ++ (v5 ++ v6) : Vec.t A (n1 + n2 + (n3 + n4 + (n5 + n6)))) ->
+  unique_vector (v1 ++ v3 ++ v5) /\ unique_vector (v2 ++ v4 ++ v6).
 Admitted.
 
-Lemma find_block_cvir :
-  forall {ni no} (ir : cvir ni no) vi vo vt bid,
-  cvir_ids_WF ir ->
-  In bid (vi ++ vt) ->
-  exists bk, find_block (blocks ir vi vo vt) bid = Some bk.
+Lemma unique_vector_build_map :
+  forall fi fo ft ni no nt,
+  (fi + ni <= fo)%nat ->
+  (fo + no <= ft)%nat ->
+  unique_vector (build_map fi ni ++ build_map fo no ++ build_map ft nt).
+Admitted.
+
+Theorem merge_cvir_relabel_WF :
+  forall ni1 no1 ni2 no2 (ir1 : cvir ni1 no1) (ir2 : cvir ni2 no2),
+  cvir_relabel_WF ir1 -> cvir_relabel_WF ir2 ->
+  cvir_relabel_WF (merge_cvir ir1 ir2).
+Proof.
+  unfold cvir_relabel_WF.
+  intros.
+  set (m := vec_build_map (vi++vo++vt) (vi'++vo'++vt')).
+  simpl in *.
+  split_vec vi ni1.
+  split_vec vo no1.
+  split_vec vt (n_int ir1).
+  split_vec vi' ni1.
+  split_vec vo' no1.
+  split_vec vt' (n_int ir1).
+  apply unique_vector_split6 in H1, H2.
+  specialize (H vi1 vi'1 vo1 vo'1 vt1 vt'1 (proj1 H1) (proj1 H2)).
+  specialize (H0 vi2 vi'2 vo2 vo'2 vt2 vt'2 (proj2 H1) (proj2 H2)).
+  rewrite 6 firstn_app_exact.
+  rewrite 6 skipn_app_exact.
+  unfold ocfg_relabel.
+  rewrite List.map_app.
+  rewrite H, H0.
+  fold (ocfg_relabel m (blocks ir1 vi1 vo1 vt1)).
+  fold (ocfg_relabel m (blocks ir2 vi2 vo2 vt2)).
+  f_equal.
+  - admit. (* the mappings are identical for the relevant keys *)
+  - admit.
+Admitted.
+
+Theorem cvir_relabel : forall {ni no} (ir : cvir ni no) vi vi' vo vo' vt vt',
+  cvir_relabel_WF ir ->
+  unique_vector (vi ++ vo ++ vt) ->
+  unique_vector (vi' ++ vo' ++ vt') ->
+  blocks ir vi' vo' vt' =
+  ocfg_relabel (vec_build_map (vi++vo++vt) (vi'++vo'++vt')) (blocks ir vi vo vt).
 Proof.
   intros.
-  eapply cvir_inputs_used in H.
-  apply find_block_in_inputs in H.
-  destruct H.
-  exists x.
-  apply H.
-  exact H0.
+  apply H; try assumption.
 Qed.
 
-(*  *)
-Theorem denote_cvir_merge : forall ni1 no1 ni2 no2 (ir1 : cvir ni1 no1) (ir2 : cvir ni2 no2) bid bid',
+Theorem eutt_cvir_relabel : forall {ni no} (ir : cvir ni no) vi vi' vo vo' vt vt' bid bid',
+  cvir_ids_WF ir ->
+  cvir_inputs_used ir ->
+  cvir_relabel_WF ir ->
+  unique_vector (vi ++ vo ++ vt) ->
+  unique_vector (vi' ++ vo' ++ vt') ->
+  eutt (ocfg_relabel_helper_rel (vec_build_map (vi++vo++vt) (vi'++vo'++vt')))
+    (denote_cvir_gen ir vi vo vt bid bid')
+    (denote_cvir_gen ir vi' vo' vt' bid bid').
+Proof.
+  intros.
+  unfold denote_cvir_gen.
+  rewrite (cvir_relabel ir vi vi' vo vo' vt vt'); try assumption.
+  erewrite <- ocfg_relabel_convert_typ.
+  apply eutt_ocfg_relabel; try assumption.
+  - apply unique_vector_app1 in H2, H3.
+    split; intro; [ apply H2 in H4 | apply H3 in H4 ]; now subst.
+  - admit. (* by definition *)
+  - admit.
+  - admit.
+  - unfold defined_map.
+    intros.
+    rewrite convert_typ_inputs in H4.
+    apply cvir_inputs in H4; try assumption.
+    apply key_in_alist_find; [ apply RelDec.RelDec_Correct_eq_typ |].
+    unfold vec_build_map.
+    rewrite combine_split.
+    + simpl. rewrite !in_app_iff. rewrite !vector_in_app_iff in H4. tauto.
+    + now rewrite 2 vector_length.
+  - unfold defined_map.
+    intros.
+    rewrite convert_typ_outputs in H4.
+    apply cvir_outputs in H4; try assumption.
+    apply key_in_alist_find; [ apply RelDec.RelDec_Correct_eq_typ |].
+    unfold vec_build_map.
+    rewrite combine_split.
+    + simpl. rewrite !in_app_iff. rewrite !vector_in_app_iff in H4. tauto.
+    + now rewrite 2 vector_length.
+  - admit.
+Admitted.
+
+Theorem denote_cvir_merge' : forall ni1 no1 ni2 no2 (ir1 : cvir ni1 no1) (ir2 : cvir ni2 no2) bid,
   cvir_ids_WF ir1 ->
   cvir_ids_WF ir2 ->
+  cvir_inputs_used ir1 ->
+  cvir_inputs_used ir2 ->
   unique_bid ir1 ->
   unique_bid ir2 ->
   eutt eq
-    (denote_cvir (merge_cvir ir1 ir2) bid bid')
+    (denote_cvir (merge_cvir ir1 ir2) bid bid)
     (match split_fin_sum ni1 ni2 bid with
-    | inl bid1 => denote_cvir ir1 bid1 bid'
-    | inr bid2 => denote_cvir ir2 bid2 bid'
+    | inl bid1 => denote_cvir_gen ir1 (build_map 0 ni1) (build_map (ni1+ni2) no1) (build_map (ni1+ni2+(no1+no2)) (n_int ir1)) bid1 bid1
+    | inr bid2 => denote_cvir_gen ir2 (build_map ni1 ni2) (build_map (ni1+ni2+no1) no2) (build_map (ni1+ni2+(no1+no2)+n_int ir1) (n_int ir2)) bid2 bid2
     end).
 Proof.
-  intros * WF11 WF12 WF21 WF22.
+  intros * WF11 WF12 WF21 WF22 WF31 WF32.
+  assert (WF3 : wf_ocfg_bid (blocks_default (merge_cvir ir1 ir2))). {
+    apply unique_bid_wf_ocfg_bid.
+    apply merge_cvir_unique; assumption.
+    admit.
+  }
+  cbn in WF3. rewrite !firstn_build_map, !skipn_build_map in WF3.
   (* case analysis on which subgraph we are in: *)
-  destruct (split_fin_sum ni1 ni2 bid) eqn:Eq. 
+  destruct (split_fin_sum ni1 ni2 bid) eqn:Eq.
   - rename f into bid1.
     unfold denote_cvir, denote_cvir_gen.
     unfold merge_cvir.
@@ -189,102 +311,142 @@ Proof.
     rewrite !firstn_build_map.
     rewrite !skipn_build_map.
     (* the invariant on the block identifiers we encounter during the computation *)
-    set (I := (fun (fto fto' : block_id * block_id) =>
-        ( exists k, snd fto' = Anon (Z.of_nat k) /\
-                    snd fto = Anon (Z.of_nat k)  /\
-                    k < ni1
-         ) \/
-        (exists k, snd fto' = Anon (Z.of_nat k) /\ 
-                   snd fto  = Anon (Z.of_nat (k + ni2 + no2)) /\ 
-                   k >= ni1 + no1 
-                   (* Need for upper bound: k < ni1 + no1 + nt1? *)
-    ))%nat).
+    (* maybe stating a higher level property on build_map or seq would be simpler? *)
+    set (I := (fun (bid bid' : block_id) =>
+      bid = bid' /\
+      exists k, bid = Anon (Z.of_nat k) /\
+      ((k >= 0 /\ k < 0+ni1) \/ (k >= ni1+ni2 /\ k < ni1+ni2+no1) \/ (k >= ni1+ni2+(no1+no2) /\ k < ni1+ni2+(no1+no2)+n_int ir1)))%nat).
+    set (I' := (fun (fto fto' : block_id * block_id) =>
+      fto = fto' /\
+      I (snd fto) (snd fto'))).
     (* we apply [eutt_iter_gen] with this invariant *)
-    apply (@KTreeFacts.eutt_iter_gen _ _ _ I). 
+    apply (@KTreeFacts.eutt_iter_gen _ _ _ I').
     + (* We need to prove that it is indeed an invariant *)
       simpl bind.
       intros [? ?b1] [? ?b2] HI.
-      destruct HI as [HI | HI].
-      * destruct HI as (k & EQ1 & EQ2 & INEQ); cbn in * |-.
-        unfold convert_typ, ConvertTyp_list, tfmap, TFunctor_list'.
-        rewrite !find_block_map' ; try auto.
-        assert (In b1 ((build_map 0 ni1) ++ (build_map (ni1 + ni2 + (no1 + no2)) (n_int ir1)))) by admit.
-        eapply find_block_cvir in H ; try assumption.
-        destruct H.
-        rewrite (find_block_some_app _ _ _ H).
-        assert (In b2 ((build_map 0 ni1) ++ (build_map (ni1 + no1) (n_int ir1)))) by admit.
-        eapply find_block_cvir in H0 ; try assumption.
-        destruct H0.
-        rewrite H0.
-        simpl.
-        (* 
-  Step 1: renaming and lookups
- 
-  find_block
-      (convert_typ nil
-         (blocks ir1 (build_map 0 ni1) (build_map (ni1 + ni2) no1)
-            (build_map (ni1 + ni2 + (no1 + no2)) (n_int ir1)) ++
-          blocks ir2 (build_map (0 + ni1) ni2)
-            (build_map (ni1 + ni2 + no1) no2)
-            (build_map (ni1 + ni2 + (no1 + no2) + n_int ir1) (n_int ir2)))%list)
-      b1 = Some bk_src1
-
-find_block
-      (convert_typ nil
-         (blocks ir1 (build_map 0 ni1) (build_map ni1 no1)
-            (build_map (ni1 + no1) (n_int ir1)))) b2 = Some bk_src2
-
-  bk_src2 = rename_bk (to_write ) bk_src1
-
-  Step 2 : correctness of renaming
-    eutt (sum_rel rename_bid eq) bk (rename_bk bk)
- *)
-        admit.
-      * admit.
-    + (* The invariant holds initially *)
-      left.
-      subst I.
-      simpl.
-      assert (proj1_sig bid = proj1_sig bid1) by admit.
-      exists (proj1_sig bid).
+      destruct HI as (? & ? & ? & ?). inv H. clear H0.
+      unfold convert_typ, ConvertTyp_list, tfmap, TFunctor_list' in *.
+      rewrite !find_block_map'; try tauto.
+      unfold option_map.
+      repeat break_match; try easy.
+      * apply find_block_app_wf in Heqo2; try assumption.
+        destruct Heqo2. 2: {
+          apply find_block_Some_In_inputs in H. destruct H1. simpl in H0. subst b2.
+          apply cvir_inputs_build_map in H; try assumption. lia.
+        }
+        rewrite H in Heqo1. inv Heqo1.
+        rewrite Heqo in Heqo0. inv Heqo0.
+        apply eutt_clo_bind with (UU := sum_rel I eq).
+        unfold denote_block.
+        apply eutt_eq_bind. intros _.
+        apply eutt_eq_bind. intros _.
+        apply eutt_translate_gen.
+        (* hard part: the terminator *)
+        assert ((forall bid, List.In bid (successors b1) -> I bid bid)). {
+          intros.
+          unfold I.
+          split; try reflexivity.
+          inv Heqo.
+          fold (ConvertTyp_block nil b3) in H0. rewrite convert_typ_successors in H0.
+          apply cvir_outputs_build_map'; try assumption.
+          eapply successors_outputs; try eassumption.
+          apply find_block_In' in H. assumption.
+        }
+        unfold successors in H0.
+        unfold denote_terminator. simpl bind.
+        intros.
+        break_match; try (apply eutt_eq_bind; tauto).
+        --break_let.
+          apply eutt_eq_bind.
+          intro.
+          apply eutt_Ret.
+          now right.
+        --apply eutt_Ret.
+          now right.
+        --break_let.
+          apply eutt_eq_bind.
+          intro.
+          apply eutt_eq_bind.
+          intro.
+          break_match; try (apply eutt_eq_bind; tauto).
+          break_match; apply eutt_Ret; left; apply H0; cbn; tauto.
+        --apply eutt_Ret. left. apply H0. cbn. tauto.
+        --admit. (* TERM_Switch *)
+        --intros.
+          repeat break_match; apply eutt_Ret; try easy.
+          ++ left. unfold I', I. inv H0. unfold I in H4. simpl. split; f_equal; tauto.
+          ++ right. now inv H0.
+      * exfalso.
+        clear Heqo Heqo0.
+        eapply find_block_app_wf in Heqo2; [| assumption ].
+        destruct Heqo2; try now rewrite H in Heqo1.
+        apply find_block_Some_In_inputs in H.
+        destruct H1. simpl in H0. inv H0.
+        apply cvir_inputs_build_map in H; try assumption. lia.
+      * eapply find_block_some_app in Heqo1.
+        now rewrite Heqo1 in Heqo2.
+      * apply eutt_Ret.
+        now right.
+    + unfold I', I.
       rewrite !nth_build_map.
-      simpl.
-      rewrite !H.
+      apply split_fin_sum_inl in Eq.
+      subst bid. destruct bid1.
       intuition.
-      apply (proj2_sig bid1).
-- admit.
+      simpl.
+      exists x.
+      intuition.
+  - admit. (* this case is similar *)
 Admitted.
 
+Theorem denote_cvir_merge1 : forall ni1 no1 ni2 no2 (ir1 : cvir ni1 no1) (ir2 : cvir ni2 no2) bid,
+  cvir_ids_WF ir1 ->
+  cvir_ids_WF ir2 ->
+  cvir_inputs_used ir1 ->
+  cvir_inputs_used ir2 ->
+  cvir_relabel_WF ir1 ->
+  cvir_relabel_WF ir2 ->
+  unique_bid ir1 ->
+  unique_bid ir2 ->
+  eutt
+    (ocfg_relabel_helper_rel (vec_build_map
+      ((build_map 0 ni1) ++ (build_map (ni1+ni2) no1) ++ (build_map (ni1+ni2+(no1+no2)) (n_int ir1)))
+      ((build_map 0 ni1) ++ (build_map ni1 no1) ++ (build_map (ni1+no1) (n_int ir1)))
+    ))
+    (denote_cvir (merge_cvir ir1 ir2) (L _ bid) (L _ bid))
+    (denote_cvir ir1 bid bid).
+Proof.
+  intros.
+  setoid_rewrite denote_cvir_merge'; try assumption.
+  break_match; rewrite split_fin_sum_L in Heqs; try discriminate.
+  inv Heqs.
+  eapply eutt_cvir_relabel; try assumption;
+  apply unique_vector_build_map; lia.
+Qed.
 
-  (*
-  clear f to FIND; intros fto fto' [-> FIND]; destruct fto as [f to] .
-  cbn in *.
-  epose proof (find_block_none_app _ bks2 _ FIND) as FIND_L1L2.
-  rewrite FIND_L1L2.
-  destruct (find_block bks2 to) eqn:FIND_L2.
-  - eapply eutt_post_bind.
-    apply denote_bk_exits_in_outputs.
-    intros [id | v] ?; cbn; apply eutt_Ret; eauto.
-    eapply inl_morphism; split; auto.
-    eapply find_block_not_in_inputs,no_reentrance_not_in; eauto.
-    eapply In_bk_outputs; eauto.
-*)
-
-(* 
-I (_, x)
-  nth vnth vi bigi bid
-
-  I : (block_id * block_id) -> (block_id * block_id) -> Prop
-  I ids1 ids2 -> eutt I ([|G1[snd ids1]|] (fst ids1)) ([|G1[snd ids2]|] (fst ids2))
-  I idsinit2 idsinit2
-  ---------
-  G1 idsinit2 ~ G2 idsinit2
-
-
-  simpl.
-  destruct (split_fin_sum _ _ _).
-Admitted.
-*)
+Theorem denote_cvir_merge2 : forall ni1 no1 ni2 no2 (ir1 : cvir ni1 no1) (ir2 : cvir ni2 no2) bid,
+  cvir_ids_WF ir1 ->
+  cvir_ids_WF ir2 ->
+  cvir_inputs_used ir1 ->
+  cvir_inputs_used ir2 ->
+  cvir_relabel_WF ir1 ->
+  cvir_relabel_WF ir2 ->
+  unique_bid ir1 ->
+  unique_bid ir2 ->
+  eutt
+    (ocfg_relabel_helper_rel (vec_build_map
+      ((build_map ni1 ni2) ++ (build_map (ni1+ni2+no1) no2) ++ (build_map (ni1+ni2+(no1+no2)+n_int ir1) (n_int ir2)))
+      ((build_map 0 ni2) ++ (build_map ni2 no2) ++ (build_map (ni2+no2) (n_int ir2)))
+    ))
+    (denote_cvir (merge_cvir ir1 ir2) (R _ bid) (R _ bid))
+    (denote_cvir ir2 bid bid).
+Proof.
+  intros.
+  setoid_rewrite denote_cvir_merge'; try assumption.
+  break_match; rewrite split_fin_sum_R in Heqs; try discriminate.
+  inv Heqs.
+  eapply eutt_cvir_relabel; try assumption;
+  apply unique_vector_build_map; lia.
+Qed.
 
 Definition sym_fin {n1 n2 n3 : nat} (f : fin (n1 + (n2 + n3))) : fin (n1 + (n3 + n2)) :=
   match split_fin_sum _ _ f with
@@ -302,15 +464,16 @@ Theorem denote_cvir_sym_i : forall {ni1 ni2 ni3 no : nat} (ir : cvir (ni1 + (ni2
   unique_bid ir ->
   eutt eq
     (denote_cvir ir bid bid')
-    (denote_cvir (sym_i_cvir ir) (sym_fin bid) bid').
+    (denote_cvir (sym_i_cvir ir) (sym_fin bid) (sym_fin bid)).
 Proof.
   intros.
   unfold denote_cvir, denote_cvir_gen, sym_i_cvir, sym_fin.
   cbn.
-  rewrite !firstn_build_map.
   rewrite !skipn_build_map.
+  rewrite !firstn_build_map.
   cbn.
   destruct (split_fin_sum _ _ _) eqn:?.
+  apply split_fin_sum_inl in Heqs. subst bid.
 Admitted.
 
 Theorem denote_cvir_relabel : forall ni no (ir : cvir ni no) vi vi' vo vo' vt vt' (bid : fin ni) bid',
@@ -323,10 +486,26 @@ Theorem denote_cvir_relabel : forall ni no (ir : cvir ni no) vi vi' vo vo' vt vt
     (denote_cvir_gen ir vi' vo' vt' bid bid').
 Admitted.
 
+(* Relation between Imp env and vellvm env *)
+
+Definition Rmem (env : Imp.env) (vmap : StringMap.t int) (venv : local_env) (vmem : memory_stack) : Prop :=
+  forall k v, alist_find k env = Some v <-> (
+    exists reg, StringMap.find k vmap = Some reg /\
+      exists addr, alist_find (Anon reg) venv = Some (UVALUE_Addr addr) /\
+        exists v32, read vmem addr (DTYPE_I (Npos 32%positive)) = inr (UVALUE_I32 v32) /\
+          Int32.intval v32 = Z.of_nat v
+  ).
+
+Definition Rimpvir
+  (vmap : StringMap.t int)
+  (env1 : Imp.env * unit)
+  (env2 : memory_stack * (local_env * (global_env * (block_id * block_id + uvalue)))) :
+  Prop :=
+  Rmem (fst env1) vmap (fst (snd env2)) (fst env2).
+
 Theorem compile_seq_correct : forall next_reg l r env next_reg' env' ir mem bid genv lenv vmem,
   compile next_reg (Seq l r) env = Some(next_reg', env', ir) ->
   eutt (Rimpvir env)
   (interp_imp (denote_imp (Seq l r)) mem)
   (interp_cfg3 (denote_cvir ir f0 bid) genv lenv vmem).
 Admitted.
-
