examples/Imp2Vir/Utils.v
@@ -1,0 +1,202 @@
+From Coq Require Import
+     Lia
+     List
+     String
+     ZArith.
+
+From ExtLib Require Import FMapAList.
+
+From ITree Require Import
+     ITree
+     ITreeFacts.
+
+From Vellvm Require Import
+     Handlers.Handlers
+     Semantics
+     Syntax
+     Syntax.ScopeTheory
+     Utils.AListFacts
+     Utils.Tactics.
+
+Open Scope nat_scope.
+
+(* Misc lemmas related to the standard library *)
+
+Lemma firstn_map : forall {A B} (l : list A) (f : A -> B) i,
+  List.firstn i (List.map f l) = List.map f (List.firstn i l).
+Proof.
+  induction l ; intros ; simpl.
+  - rewrite 2 List.firstn_nil.
+    reflexivity.
+  - destruct i.
+    + reflexivity.
+    + simpl. rewrite <- IHl.
+      reflexivity.
+Qed.
+
+Lemma firstn_seq : forall n n' i, List.firstn n (List.seq i (n + n')) = List.seq i n.
+Proof.
+  induction n ; intros ; simpl.
+  - reflexivity.
+  - f_equal.
+    rewrite IHn.
+    reflexivity.
+Qed.
+
+Lemma skipn_map : forall {A B} (l : list A) (f : A -> B) i,
+  List.skipn i (List.map f l) = List.map f (List.skipn i l).
+Proof.
+  induction l ; intros ; simpl.
+  - rewrite 2 List.skipn_nil.
+    reflexivity.
+  - destruct i.
+    + reflexivity.
+    + simpl. rewrite <- IHl.
+      reflexivity.
+Qed.
+
+Lemma skipn_seq : forall n n' i, List.skipn n (List.seq i (n + n')) = List.seq (i + n) n'.
+Proof.
+  induction n ; intros ; simpl.
+  - auto.
+  - destruct n'.
+    + simpl.
+      apply skipn_all2.
+      rewrite seq_length.
+      lia.
+    + simpl.
+      rewrite IHn. simpl.
+      f_equal; auto.
+Qed.
+
+Lemma find_app :
+  forall {A} (l1 l2 : list A) f x,
+  List.find f (l1 ++ l2) = Some x ->
+  List.find f l1 = Some x \/ List.find f l2 = Some x.
+Proof.
+  intros.
+  induction l1.
+  - now right.
+  - simpl in *.
+    break_match; tauto.
+Qed.
+
+(* Misc lemmas related to extlib *)
+
+Lemma key_in_alist_find : forall {A B : Type} {RD : RelDec.RelDec eq},
+  RelDec.RelDec_Correct RD ->
+  forall (l : alist A B) k,
+  List.In k (fst (split l)) ->
+  exists v, alist_find k l = Some v.
+Proof.
+  intros.
+  induction l; [ destruct H0 |].
+  cbn in *. repeat break_let. subst.
+  cbn in *.
+  destruct H0.
+  - subst.
+    exists b.
+    break_match; try easy.
+    now apply RelDec.neg_rel_dec_correct in Heqb0.
+  - apply IHl in H0 as [].
+    break_match.
+    + now exists b.
+    + now exists x.
+Qed.
+
+(* Misc lemmas related to vellvm *)
+
+(* The following three are copied from vellvm,
+   but with heterogeneous types T and T' for use with convert_typ *)
+
+Lemma find_block_map_some' :
+  forall {T T'} (f : block T -> block T') G b bk,
+    (forall bk, blk_id (f bk) = blk_id bk) ->
+    find_block G b = Some bk ->
+    find_block (List.map f G) b = Some (f bk).
+Proof.
+  intros * ID; induction G as [| hd G IH]; intros FIND ; [inv FIND |].
+  cbn in *.
+  rewrite ID.
+  break_match_goal; break_match_hyp; intuition.
+  inv FIND; auto.
+Qed.
+
+Lemma find_block_map_none' :
+  forall {T T'} (f : block T -> block T') G b,
+    (forall bk, blk_id (f bk) = blk_id bk) ->
+    find_block G b = None ->
+    find_block (List.map f G) b = None.
+Proof.
+  intros * ID; induction G as [| hd G IH]; intros FIND; [reflexivity |].
+  cbn in *.
+  rewrite ID.
+  break_match_goal; break_match_hyp; intuition.
+  inv FIND; auto.
+Qed.
+
+Lemma find_block_map' :
+  forall {T T'} (f : block T -> block T') G b,
+    (forall bk, blk_id (f bk) = blk_id bk) ->
+    find_block (List.map f G) b = option_map f (find_block G b).
+Proof.
+  intros.
+  destruct (find_block G b) eqn:EQ.
+  eapply find_block_map_some' in EQ; eauto.
+  eapply find_block_map_none' in EQ; eauto.
+Qed.
+
+Lemma find_block_app_wf :
+  forall {T : Set} (x : block_id) [b : block T] (bs1 bs2 : ocfg T),
+  wf_ocfg_bid (bs1 ++ bs2)%list ->
+  find_block (bs1 ++ bs2) x = Some b ->
+  find_block bs1 x = Some b \/ find_block bs2 x = Some b .
+Proof.
+  intros.
+  unfold find_block in H0.
+  now apply find_app.
+Qed.
+
+Lemma outputs_successors : forall {typ} (cfg : ocfg typ) o,
+  List.In o (outputs cfg) ->
+  exists bk, List.In bk cfg /\ List.In o (successors bk).
+Proof.
+  induction cfg; intros.
+  - destruct H.
+  - cbn in H. rewrite outputs_acc in H.
+    apply List.in_app_iff in H. destruct H.
+    + exists a. simpl. tauto.
+    + apply IHcfg in H.
+      destruct H. exists x.
+      simpl. tauto.
+Qed.
+
+Lemma successors_outputs : forall {typ} (cfg : ocfg typ) o bk,
+  List.In bk cfg ->
+  List.In o (successors bk) ->
+  List.In o (outputs cfg).
+Proof.
+  induction cfg; intros.
+  - destruct H.
+  - cbn. rewrite outputs_acc.
+    apply List.in_app_iff.
+    destruct H.
+    + left. now subst a.
+    + right. apply IHcfg in H0; assumption.
+Qed.
+
+Lemma convert_typ_inputs : forall bk,
+  inputs (convert_typ nil bk) = inputs bk.
+Proof.
+  intros.
+  unfold inputs, convert_typ, ConvertTyp_list, tfmap, TFunctor_list'.
+  rewrite List.map_map.
+  reflexivity.
+Qed.
+
+Lemma convert_typ_successors : forall (bk : block typ),
+  successors (convert_typ nil bk) = successors bk.
+Proof.
+  intros.
+  apply convert_typ_terminator_outputs.
+Qed.
